WIP

demo/fib/FibS01proof.v
@@ -132,24 +132,179 @@ Proof.
   exploit H0; et. i. eauto with paco.
 Qed.
 
+Global Instance sim_st_Reflexive n: Reflexive (sim_st n).
+Proof.
+  rr. revert n.
+  ginit.
+  { intros. eapply cpn3_wcompat; eauto with paco. }
+  gcofix CIH. ii. gstep.
+  ides x.
+  - destruct r0 as [oh [m vs]]. econs; et.
+  - econs; et. eauto with paco.
+  - destruct e.
+    + destruct e. econs; et. ii. rr in H. des_ifs. des; clarify. eauto with paco.
+    + destruct e.
+      * econs.
+      * econs.
+      * econs; et. ii. esplits; et. eauto with paco.
+Unshelve.
+  all: ss.
+Qed.
+
 Definition rclo: (state owned_heap) -> (state owned_heap) -> Prop :=
   rtc ((sim_st 0%nat) \2/ eutt eq).
+
+Inductive rtcn A (R: A -> A -> Prop): forall (n:nat) (a1 a2:A), Prop :=
+| rtcn_nil
+    a:
+    rtcn R 0 a a
+| rtcn_cons
+    a1 a2 a3 n
+    (A12: R a1 a2)
+    (A23: rtcn R n a2 a3):
+    rtcn R (S n) a1 a3
+.
+Hint Constructors rtcn.
+
+Lemma rtcn_rtc A (R: A -> A -> Prop) n a1 a2
+      (RTCN: rtcn R n a1 a2):
+  rtc R a1 a2.
+Proof.
+  induction RTCN; auto. econs; eauto.
+Qed.
+
+Lemma rtc_rtcn A (R: A -> A -> Prop) a1 a2
+      (RTC: rtc R a1 a2):
+  exists n, rtcn R n a1 a2.
+Proof.
+  induction RTC; eauto. i. des.
+  esplits; eauto.
+Qed.
+
+Definition rcloN: nat -> (state owned_heap) -> (state owned_heap) -> Prop :=
+  fun n => rtcn ((sim_st 0%nat) \2/ eutt eq) n.
+
+(* Axiom A B: Type. *)
+(* Axiom P: A -> (nat -> B) -> Prop. *)
+(* Goal (forall a: A, exists b: (nat -> B), P a b) -> (exists b: (nat -> B), forall a, P a b). *)
+(* Proof. *)
+(*   i. *)
+(* Qed. *)
+
+Lemma rclo_bind_aux_aux
+      n m
+      k0 k1
+      (K: (eq ==> rcloN n) k0 k1)
+      i0 i1
+      (H: rcloN m i0 i1)
+  :
+    rcloN (n + m)%nat (t <- i0;; k0 t) (t <- i1;; k1 t)
+.
+Proof.
+  ginduction n; ii; ss.
+  - assert(k0 = k1).
+    { apply func_ext1. intro. exploit (K x0); et. intro T. inv T. ss. }
+    subst. clear K.
+    ginduction m; ii; ss.
+    + inv H. econs; et.
+    + inv H. des.
+      { econs; et.
+        - left. eapply sim_st_bind; et. ii. clarify. refl.
+        - eapply IHm; et. }
+      { econs; et.
+        - right. eapply eutt_eq_bind; et. ii. clarify. refl.
+        - eapply IHm; et. }
+  -
+    (* assert(exists km, <<A: forall x, rclo (k0 x) (km x)>> *)
+    (*                                  /\ <<B: forall x, rcloN n (km x) (k1 x)>>). *)
+    (* { clear - K. r in K. *)
+    (*   exists (fun _ => _). *)
+    (*   admit "". } *)
+    econs; et; cycle 1.
+    + eapply IHn; et.
+Abort.
+
+Lemma rclo_bind_aux_aux
+      n m
+      k0 k1
+      (K: rtcn (fun f0 f1 => (forall x, sim_st 0 (f0 x) (f1 x)) \/
+                             (forall x, eutt eq (f0 x) (f1 x))) n k0 k1)
+      i0 i1
+      (H: rcloN m i0 i1)
+  :
+    rcloN (n + m)%nat (t <- i0;; k0 t) (t <- i1;; k1 t)
+.
+Proof.
+  ginduction n; ii; ss.
+  - inv K.
+    ginduction m; ii; ss.
+    + inv H. econs; et.
+    + inv H. des.
+      { econs; et.
+        - left. eapply sim_st_bind; et. ii. clarify. refl.
+        - eapply IHm; et. }
+      { econs; et.
+        - right. eapply eutt_eq_bind; et. ii. clarify. refl.
+        - eapply IHm; et. }
+  - inv K.
+    econs; et; cycle 1.
+    + eapply IHn; et.
+    + des.
+      { left. eapply sim_st_bind; et.
+        - ii. clarify.
+        - refl.
+      }
+      { right. eapply eutt_eq_bind; et. refl. }
+Qed.
+
+
+
+Lemma rclo_bind_aux
+      k0 k1
+      (K: (eq ==> rclo) k0 k1)
+      i0 i1
+      (H: rclo i0 i1)
+  :
+    rclo (t <- i0;; k0 t) (t <- i1;; k1 t)
+.
+Proof.
+  eapply rtc_rtcn in H. des.
+  assert(T: exists max, forall ohmv, rcloN max (k0 ohmv) (k1 ohmv)).
+  { admit "". }
+  des.
+  eapply rtcn_rtc.
+  eapply rclo_bind_aux_aux; et.
+  instantiate (1:= max).
+  clear - T.
+  ginduction max; ii; ss.
+  { assert(k0 = k1).
+    { eapply func_ext1. ii. exploit T; et. intro U. inv U. et. }
+    subst. econs; et.
+  }
+  econs; et.
+Abort.
 
 Global Instance rclo_bind: Proper ((eq ==> rclo) ==> rclo ==> rclo) (ITree.bind').
 Proof.
   ii.
   rename x0 into i0. rename y0 into i1.
   rename x into k0. rename y into k1.
-  assert(LEMMA: forall x (k0 k1: owned_heap * (mem * val) -> state owned_heap),
-            ((eq ==> rclo) k0 k1) -> rclo (` x : _ <- x;; k0 x) (` x : _ <- x;; k1 x)).
-  { admit "". }
-  move LEMMA at top. move H0 at top.
-  revert_until LEMMA.
   induction H0; ii; ss; et.
-  fold rclo in H0.
-  etrans; cycle 1.
-  { eapply IHclos_refl_trans_1n; eauto. }
-  clears z. clear z. clears k1. clear k1.
+  - assert(exists max, forall x, rcloN max (k0 x) (k1 x)).
+    { admit "". }
+    des. clear H.
+    ginduction max; ii; ss.
+    + assert(k0 = k1).
+      { apply func_ext1. ii. exploit H0; et. intro T. inv T; et. }
+      subst. refl.
+    + admit "".
+  - etrans; cycle 1.
+    { eapply IHclos_refl_trans_1n; eauto. }
+    des.
+    + eapply rtc_n1; et.
+      { left. eapply sim_st_bind; et. ii. clarify. refl. }
+    + eapply rtc_n1; et.
+      { right. eapply eutt_eq_bind; et. ii. clarify. refl. }
 Abort.
 
 
@@ -192,54 +347,54 @@ Qed.
 
 
 
-Lemma unfold_fib2: forall oh0 m0 vs0,
-    sim_st 0%nat (interp_mrec (interp_function FibS0.prog) (FibS0.f_fib oh0 m0 vs0))
-      (`n: nat <- (unwrapU (parse_arg oh0 m0 vs0)) ;;
-    match n with
-    | O => Ret (oh0, (m0, (Vint Int.zero)))
-    | S O => Ret (oh0, (m0, (Vint Int.one)))
-    | S (S m) =>
-      let vs0 := [Vint (of_nat m)] in
-      guarantee (parse_arg oh0 m0 vs0) ;;
-      tau;;
-      '(oh1, (m1, y1)) <- (interp_mrec (interp_function FibS0.prog) (FibS0.f_fib oh0 m0 vs0)) ;;
+(* Lemma unfold_fib2: forall oh0 m0 vs0, *)
+(*     sim_st 0%nat (interp_mrec (interp_function FibS0.prog) (FibS0.f_fib oh0 m0 vs0)) *)
+(*       (`n: nat <- (unwrapU (parse_arg oh0 m0 vs0)) ;; *)
+(*     match n with *)
+(*     | O => Ret (oh0, (m0, (Vint Int.zero))) *)
+(*     | S O => Ret (oh0, (m0, (Vint Int.one))) *)
+(*     | S (S m) => *)
+(*       let vs0 := [Vint (of_nat m)] in *)
+(*       guarantee (parse_arg oh0 m0 vs0) ;; *)
+(*       tau;; *)
+(*       '(oh1, (m1, y1)) <- (interp_mrec (interp_function FibS0.prog) (FibS0.f_fib oh0 m0 vs0)) ;; *)
 
-      let vs1 := [Vint (of_nat (S m))] in
-      guarantee (parse_arg oh1 m1 vs1) ;;
-      tau;;
-      '(oh2, (m2, y2)) <-  (interp_mrec (interp_function FibS0.prog) (FibS0.f_fib oh1 m1 vs1)) ;;
+(*       let vs1 := [Vint (of_nat (S m))] in *)
+(*       guarantee (parse_arg oh1 m1 vs1) ;; *)
+(*       tau;; *)
+(*       '(oh2, (m2, y2)) <-  (interp_mrec (interp_function FibS0.prog) (FibS0.f_fib oh1 m1 vs1)) ;; *)
 
-      Ret (oh2, (m2, Vint (of_nat (fib_nat n))))
-    end
-      )
-.
-Proof.
-  {
-    i. irw.
-    unfold FibS0.f_fib at 2. irw.
-    unfold unwrapU. des_ifs; cycle 1.
-    { unfold triggerUB. irw. pfold. econs; et. }
-    irw. destruct n.
-    { irw. pfold. econs; et. }
-    destruct n.
-    { irw. pfold. econs; et. }
-    destruct (to_nat_opt (of_nat n)) eqn:T; ss; cycle 1.
-    { unfold guarantee. des_ifs_safe. irw. unfold triggerNB. irw. pfold. econs; et. }
-    unfold guarantee. des_ifs_safe. irw. pfold. econs; et. left.
-    des_ifs_safe.
-    rewrite <- ! unfold_interp_mrec.
-    rewrite interp_mrec_bind. f_equiv; cycle 1.
-    { (*** TODO: prove reflexive, or we may just use rtc of sim_st ***)
-      admit "refl".
-    }
-    ii. des_ifs; cycle 1.
-    { irw. unfold triggerNB. irw. pfold. econs; et. }
-    rewrite ! bind_ret_l.
-    rewrite interp_mrec_bind. irw. pfold. econs; et. left. f_equiv.
-    { ii. clarify. irw. des_ifs. ss. pfold. econs; et. }
-    { des_ifs. irw. admit "refl". }
-  }
-Qed.
+(*       Ret (oh2, (m2, Vint (of_nat (fib_nat n)))) *)
+(*     end *)
+(*       ) *)
+(* . *)
+(* Proof. *)
+(*   { *)
+(*     i. irw. *)
+(*     unfold FibS0.f_fib at 2. irw. *)
+(*     unfold unwrapU. des_ifs; cycle 1. *)
+(*     { unfold triggerUB. irw. pfold. econs; et. } *)
+(*     irw. destruct n. *)
+(*     { irw. pfold. econs; et. } *)
+(*     destruct n. *)
+(*     { irw. pfold. econs; et. } *)
+(*     destruct (to_nat_opt (of_nat n)) eqn:T; ss; cycle 1. *)
+(*     { unfold guarantee. des_ifs_safe. irw. unfold triggerNB. irw. pfold. econs; et. } *)
+(*     unfold guarantee. des_ifs_safe. irw. pfold. econs; et. left. *)
+(*     des_ifs_safe. *)
+(*     rewrite <- ! unfold_interp_mrec. *)
+(*     rewrite interp_mrec_bind. f_equiv; cycle 1. *)
+(*     { (*** TODO: prove reflexive, or we may just use rtc of sim_st ***) *)
+(*       admit "refl". *)
+(*     } *)
+(*     ii. des_ifs; cycle 1. *)
+(*     { irw. unfold triggerNB. irw. pfold. econs; et. } *)
+(*     rewrite ! bind_ret_l. *)
+(*     rewrite interp_mrec_bind. irw. pfold. econs; et. left. f_equiv. *)
+(*     { ii. clarify. irw. des_ifs. ss. pfold. econs; et. } *)
+(*     { des_ifs. irw. admit "refl". } *)
+(*   } *)
+(* Qed. *)
 
 Lemma unfold_fib3: forall oh0 m0 vs0,
     (interp_mrec (interp_function FibS0.prog) (FibS0.f_fib oh0 m0 vs0))
@@ -347,62 +502,11 @@ Proof.
   destruct (to_nat_opt (of_nat n)) eqn:U; cycle 1.
   { des_ifs_safe. unfold triggerNB. irw. pfold. econs; et. }
   ss. des_ifs_safe. irw.
-  ------------------------------------
-  pfold.
-  irw.
-  ss.
-  destruct (to_nat_opt (of_nat n)) eqn:U; cycle 1.
-  { des_ifs_safe. unfold triggerNB. irw. pfold. econs; et. }
-  
-  unfold guarantee. des_ifs.
-  unfold unwrapU, parse_arg. rewrite T. ss. rewrite bind_ret_l.
-  unfold guarantee. destruct (to_nat_opt (of_nat n)) eqn:U; cycle 1.
-  { des_ifs_safe. unfold triggerNB. irw. pfold. econs; et. }
-  ss. des_ifs_safe. rewrite bind_ret_l.
-  assert(n = n0).
-  { unfold to_nat_opt, of_nat in U. des_ifs. rewrite Int.signed_repr.
-    - rewrite Nat2Z.id. ss.
-    - admit "more integer reasoning from below facts needed".
-  }
-  subst.
-  rewrite fib_nat_recurse.
-  eapply rtc_n1; cycle 1.
-  { right. rewrite ! tau_eutt. refl. }
-  fold rel_trans.
-
-
-  unfold f_fib. unfold unwrapU. rewrite unfold_interp_mrec. ss. des_ifs_safe. rewrite ! bind_ret_l. ss.
-  rewrite <- H; cycle 1.
-  { instantiate (1:= n). eauto. }
-  { ss. }
-  unfold f_fib. unfold unwrapU. rewrite unfold_interp_mrec. ss. des_ifs. repeat (rewrite bind_ret_l; ss).
-  rewrite <- H; cycle 1.
-  { instantiate (1:= S n). eauto. }
-  { ss. }
-  unfold f_fib. ss. unfold unwrapU. des_ifs. ss. rewrite bind_ret_l.
-  rewrite unfold_interp_mrec. ss. rewrite bind_ret_l.
-  refl.
-
-
-
-
-
-  unfold f_fib. unfold unwrapU. des_ifs.rewrite unfold_interp_mrec. ss. des_ifs; cycle 1.
-  { irw. eapply rtc_once. left. unfold triggerNB. irw. pfold. econs; et. }
-  rewrite ! bind_ret_l. ss.
-  rewrite <- H; cycle 1.
-  { instantiate (1:= n). eauto. }
-  { ss. }
-  unfold f_fib. unfold unwrapU. rewrite unfold_interp_mrec. ss. des_ifs. repeat (rewrite bind_ret_l; ss).
-  rewrite <- H; cycle 1.
-  { instantiate (1:= S n). eauto. }
-  { ss. }
-  unfold f_fib. ss. unfold unwrapU. des_ifs. ss. rewrite bind_ret_l.
-  rewrite unfold_interp_mrec. ss. rewrite bind_ret_l.
-  refl.
-  econs.
-  pfold.
+  admit "----------------------------------------------------------------------".
+Unshelve.
+  all: try econs.
 Qed.
+Local Transparent prog FibS0.prog.
 
 Theorem lemma
         m vs oh
@@ -418,85 +522,19 @@ Theorem lemma
 Proof.
   destruct (parse_arg oh m vs) eqn:T; cycle 1.
   { unfold interp_program, mrec. irw. des_ifs.
+    cbn in *.
     unfold f_fib at 2. unfold FibS0.f_fib at 2.
     unfold unwrapU. des_ifs. irw. pfold; econs; et.
   }
   clear_tac.
   eapply lemma_aux; et.
-
-  move n at top. revert_until n.
-  pattern n. eapply well_founded_ind.
-  { eapply lt_wf. }
-  clear n. intros.
-  rename x into n.
-
-  destruct n.
-  { unfold parse_arg in *. des_ifs.
-    unfold interp_program, mrec. ss. des_ifs. cbn in Heq, Heq0. des_ifs. clear_tac.
-    rewrite ! unfold_interp_mrec.
-    unfold f_fib, FibS0.f_fib. ss. rewrite T. ss. irw. Fail refl. pfold. econs; et. }
-  destruct n.
-  { unfold parse_arg in *. des_ifs.
-    unfold interp_program, mrec. ss. des_ifs. cbn in Heq, Heq0. des_ifs. clear_tac.
-    rewrite ! unfold_interp_mrec.
-    unfold f_fib, FibS0.f_fib. ss. rewrite T. ss. irw. Fail refl. pfold. econs; et. }
-
-  unfold parse_arg in T. des_ifs.
-  unfold interp_program, mrec. ss. des_ifs. cbn in Heq, Heq0. des_ifs. clear_tac.
-  rewrite unfold_fib3. unfold unwrapU, parse_arg. rewrite T. ss. rewrite bind_ret_l.
-  unfold guarantee. destruct (to_nat_opt (of_nat n)) eqn:U; cycle 1.
-  { des_ifs_safe. unfold triggerNB. irw. pfold. econs; et. }
-  ss. des_ifs_safe. rewrite bind_ret_l.
-  assert(n = n0).
-  { unfold to_nat_opt, of_nat in U. des_ifs. rewrite Int.signed_repr.
-    - rewrite Nat2Z.id. ss.
-    - admit "more integer reasoning from below facts needed".
-  }
-  subst.
-  rewrite fib_nat_recurse.
-  eapply rtc_n1; cycle 1.
-  { right. rewrite ! tau_eutt. refl. }
-  fold rel_trans.
-
-
-  unfold f_fib. unfold unwrapU. rewrite unfold_interp_mrec. ss. des_ifs_safe. rewrite ! bind_ret_l. ss.
-  rewrite <- H; cycle 1.
-  { instantiate (1:= n). eauto. }
-  { ss. }
-  unfold f_fib. unfold unwrapU. rewrite unfold_interp_mrec. ss. des_ifs. repeat (rewrite bind_ret_l; ss).
-  rewrite <- H; cycle 1.
-  { instantiate (1:= S n). eauto. }
-  { ss. }
-  unfold f_fib. ss. unfold unwrapU. des_ifs. ss. rewrite bind_ret_l.
-  rewrite unfold_interp_mrec. ss. rewrite bind_ret_l.
-  refl.
-
-
-
-
-
-  unfold f_fib. unfold unwrapU. des_ifs.rewrite unfold_interp_mrec. ss. des_ifs; cycle 1.
-  { irw. eapply rtc_once. left. unfold triggerNB. irw. pfold. econs; et. }
-  rewrite ! bind_ret_l. ss.
-  rewrite <- H; cycle 1.
-  { instantiate (1:= n). eauto. }
-  { ss. }
-  unfold f_fib. unfold unwrapU. rewrite unfold_interp_mrec. ss. des_ifs. repeat (rewrite bind_ret_l; ss).
-  rewrite <- H; cycle 1.
-  { instantiate (1:= S n). eauto. }
-  { ss. }
-  unfold f_fib. ss. unfold unwrapU. des_ifs. ss. rewrite bind_ret_l.
-  rewrite unfold_interp_mrec. ss. rewrite bind_ret_l.
-  refl.
-  econs.
-  pfold.
 Qed.
 
 Theorem correct: rusc defaultR [FibS1.module: Mod.t] [FibS0.module: Mod.t].
 Proof.
   eapply SimSIR.correct; ss.
-  econs; try apply unit_ord_wf; ss.
-  ii. clarify. exists tt.
+  econs; try apply lt_wf; ss.
+  ii. clarify. exists O.
   r.
   destruct (ident_eq fname Fib0._fib); cycle 1.
   { unfold interp_program, mrec. irw. des_ifs. irw. pfold. econs; et. }
@@ -514,106 +552,5 @@ Proof.
   clear n. intros.
   rename x into n.
 
-  destruct n.
-  { unfold parse_arg in *. des_ifs.
-    unfold interp_program, mrec. ss. des_ifs. cbn in Heq, Heq0. des_ifs. clear_tac.
-    rewrite ! unfold_interp_mrec.
-    unfold f_fib, FibS0.f_fib. ss. rewrite T. ss. irw. pfold. econs; et. }
-  destruct n.
-  { unfold parse_arg in *. des_ifs.
-    unfold interp_program, mrec. ss. des_ifs. cbn in Heq, Heq0. des_ifs. clear_tac.
-    rewrite ! unfold_interp_mrec.
-    unfold f_fib, FibS0.f_fib. ss. rewrite T. ss. irw. pfold. econs; et. }
-
-  unfold parse_arg in T. des_ifs.
-  unfold interp_program, mrec. ss. des_ifs. cbn in Heq, Heq0. des_ifs. clear_tac.
-  rewrite unfold_fib3. unfold unwrapU, parse_arg. rewrite T. ss. rewrite bind_ret_l.
-  unfold guarantee. destruct (to_nat_opt (of_nat n)) eqn:U; cycle 1.
-  { des_ifs_safe. unfold triggerNB. irw. pfold. econs; et. }
-  ss. des_ifs_safe. rewrite bind_ret_l.
-  assert(n = n0).
-  { unfold to_nat_opt, of_nat in U. des_ifs. rewrite Int.signed_repr.
-    - rewrite Nat2Z.id. ss.
-    - admit "more integer reasoning from below facts needed".
-  }
-  subst. irw. pfold.
-
-  rewrite U.
-  assert(U: to_nat_opt (of_nat n) = Some n).
-  { admit "should be derived from guarantee". }
-  unfoldr guarantee. rewrite U. ss. des_ifs_safe. rewrite bind_ret_l.
-  assert(V: to_nat_opt (of_nat (S n)) = Some (S n)).
-  { admit "should be derived from guarantee". }
-  des_ifs. unfold guarantee. rewrite V. ss. des_ifs.
-  setoid_rewrite <- H; cycle 1.
-  { instantiate (1:= n). eauto. }
-  { ss. }
-  unfold f_fib. unfold unwrapU. rewrite unfold_interp_mrec. ss. des_ifs.
-  rewrite ! bind_ret_l. ss.
-  rewrite unfold_interp_mrec. ss. rewrite ! bind_ret_l.
-  rewrite <- H; cycle 1.
-  { instantiate (1:= S n). eauto. }
-  { ss. }
-  unfold f_fib. ss. rewrite V. ss. rewrite bind_ret_l.
-  rewrite unfold_interp_mrec. ss. rewrite bind_ret_l. refl.
-
-
-  { irw. unfold interp_program, mrec. irw. des_ifs. unfold f_fib, FibS0.f_fib. irw.
-
-  ginduction n; ii; ss.
-  { unfold parse_arg in *. des_ifs. irw.
-    unfold interp_program, mrec. irw. des_ifs.
-    unfold f_fib at 2. unfold FibS0.f_fib at 2.
-    irw. unfold to_nat_opt in *. des_ifs. irw. des_ifs. irw. pfold. econs; et. }
-  unfold parse_arg in T. des_ifs_safe.
-  unfold interp_program, mrec. irw. des_ifs.
-  unfold f_fib at 2. unfold FibS0.f_fib at 2. irw.
-  my_tac. unfold unwrapU. des_ifs. irw.
-  des_ifs.
-  { pfold. econs; et. }
-  rewrite ! range_to_nat; cycle 1.
-  { admit "int reasoning". }
-  { admit "int reasoning". }
-  unfold guarantee. des_ifs; cycle 1. clear_tac.
-  irw.
-  assert(BDOOR: forall E R (it: itree E R), (tau;; it) = it).
-  { admit "". }
-  rewrite BDOOR.
-  des_ifs.
-  rewrite <- unfold_interp_mrec.
-Abort.
-
-
-
-Theorem correct: rusc defaultR [FibS1.module: Mod.t] [FibS0.module: Mod.t].
-Proof.
-  eapply SimSIR.correct; ss.
-  econs; try apply unit_ord_wf; ss.
-  ii. clarify. exists tt.
-  r. unfold interp_program, mrec. irw.
-  destruct (ident_eq fname Fib0._fib); cycle 1.
-  { des_ifs. irw. pfold. econs; et. }
-  clarify. des_ifs. clear_tac.
-  repeat match goal with
-  | [ |- context[interp_function ?H] ] =>
-    let name := fresh "x" in set (name := (interp_function H)) in *
-  end
-  .
-  unfold f_fib. irw.
-  unfold FibS0.f_fib. irw.
-  unfold unwrapU. des_ifs; cycle 1.
-  { irw. pfold. econs; et. }
-  rename Heq into T.
-  irw.
-  revert T.
-  revert oh_tgt.
-  revert vs.
-  revert m.
-  induction n; ii; ss.
-  { unfold parse_arg in *. des_ifs. irw. pfold. econs; et. }
-  unfold parse_arg in *. des_ifs_safe.
-  destruct n.
-  { irw. pfold. econs; et. }
-  eapply sim_st_trans; cycle 1.
-  {
-Abort.
+  eapply lemma.
+Qed.
